EggTactic/Tracing.lean
@@ -1,0 +1,2 @@
+import Lean
+initialize Lean.registerTraceClass `EggTactic.egg
